Language_Components/Imp_Ctl/Imp_Ctl.thy
@@ -64,7 +64,7 @@ definition imp_sem_lifting_gen :: "(syn', 'x imp_state',
                                    ('x, _ ) state) lifting" where
 "imp_sem_lifting_gen = 
  (schem_lift (SP NA NB)
-             (SP (SPRC imp_prio (SO NA)) (SP NX (SP (SPRK (SO NB)) NX))))"
+             (SP (SPRC imp_prio (SO NA)) (SP NX (SP (SPRI (SO NB)) NX))))"
 
 
 definition imp_sem_l_gen :: "('s \<Rightarrow> syn') \<Rightarrow> 's \<Rightarrow> ('x, 'z :: Mergeableb) state \<Rightarrow> ('x, 'z) state" where
