Languages/Imp/Calc_Mem_Imp.thy
@@ -1,4 +1,7 @@
-theory Calc_Mem_Imp imports Calc_Mem "../../Language_Components/Cond/Cond" 
+theory Calc_Mem_Imp imports (*Calc_Mem*)
+ "../../Language_Components/Cond/Cond" 
+ "../../Language_Components/Calc/Calc"
+  "../../Language_Components/Mem/Mem_Simple"
               "../../Language_Components/Imp_Ctl/Imp_Ctl" 
              "../../Language_Components/Seq/Seq" 
 "../../Hoare/Hoare_Step"
@@ -77,6 +80,17 @@ definition calc_sem_l :: "syn \<Rightarrow> ('s, _) state \<Rightarrow> ('s, _) 
        'c::{Bogus,Pord}) lifting
 *)
 
+definition baseline_l where
+"baseline_l =
+  schem_lift (SP NA (SP NB (SP NC (SP ND (SP NE (SP NF (SP NG NH)))))))
+  (SP (SPRI (SO NA)) (SP (SPRI (SO NB)) (SP (SPRI (SO NC)) (SP (SPRI (SO ND)) (SP (SPRI (SO NE)) 
+    (SP (SPRI (SO NF)) (SP (SPRI (SO NG)) (SID NH))))))))"
+
+definition baseline_f where
+"baseline_f =
+  LMap baseline_l (\<lambda> _ . id)"
+
+term "baseline_f id"
 term "no_control_lifting (schem_lift (SP NA (SP NB NC)) (SP (SPRI (SO NC)) (SP (SPRI (SO NB)) (SP (SPRI (SO NA)) NX ))))"
 term "no_control_lifting"
 
@@ -87,13 +101,30 @@ definition calc_schemi where
 "calc_schemi = (SP NA (SP NB NC))"
 declare calc_schemi_def [simp]
 
+definition calc_lift_aux1 where
+"calc_lift_aux1 = 
+  schem_lift NA (SPRI (SO NA))"
+declare calc_lift_aux1_def [simp]
+
+definition calc_lift_aux2 where
+"calc_lift_aux2 =
+  schem_lift NA (SP (SPRI (SO NA)) NX)"
+
 definition calc_schemo where
-"calc_schemo = (SP NX (SP (SPRC calc_prio (SO NC)) (SP (SPRI (SO NA)) (SP (SPRI (SO NB)) NX ))))"
+"calc_schemo = (SP NX (SP (SPRC calc_prio (SO NC)) (SP (SPRI (SO NA)) (SP (SPRI (SO NB)) NX))))"
 declare calc_schemo_def [simp]
 
 definition calc_lift :: "(Calc.calc, Calc.calc_state, ('s, 'x :: {Bogus, Pord, Mergeableb, Okay}) Mem_Simple.state) lifting" where
 "calc_lift = 
   no_control_lifting (schem_lift calc_schemi calc_schemo)"
+
+term "(schem_lift calc_schemi calc_schemo)"
+
+definition with_baseline :: 
+  "(syn \<Rightarrow> ('s, _) state \<Rightarrow> ('s, _) state) \<Rightarrow>
+   (syn \<Rightarrow> ('s, _) state \<Rightarrow> ('s, _) state)" where
+"with_baseline f syn st =
+  [^f syn st, baseline_f syn st^]"
 
 (* TODO: priority stuff is all wrong here. *)
 (* concretize our schem_lift at an appropriate type. *)
@@ -111,7 +142,8 @@ definition mem_sem_l :: "syn \<Rightarrow> ('s, _) state \<Rightarrow> ('s, _) s
 *)
 definition cond_lift where
 "cond_lift = 
-  no_control_lifting (schem_lift (SP NA NB) (SP (SPRC cond_prio (SO NA)) (SP (SPRI (SO NB)) NX)))"
+  no_control_lifting (schem_lift (SP NA NB) (SP (SPRC cond_prio (SO NA)) 
+                     (SP (SPRI (SO NB)) NX)))"
 
 definition cond_sem_l :: "syn \<Rightarrow> ('s, _) state \<Rightarrow> ('s, _) state" where
 "cond_sem_l =
@@ -134,7 +166,7 @@ definition mem_sem_l :: "syn \<Rightarrow> ('s, _) state \<Rightarrow> ('s, _) s
 
 definition sem_final :: "syn \<Rightarrow> ('s, (_ :: Pordc_all)) state \<Rightarrow> ('s, (_ :: Pordc_all)) state" where
 "sem_final =
-  pcomps [calc_sem_l, mem_sem_l, cond_sem_l, imp_sem_l, seq_sem_l]"
+  pcomps [with_baseline calc_sem_l, with_baseline mem_sem_l, with_baseline cond_sem_l, with_baseline imp_sem_l, with_baseline seq_sem_l]"
 
 definition sems ::
   "(syn \<Rightarrow> ('s, (_ :: Pordc_all)) state \<Rightarrow> ('s, (_ :: Pordc_all)) state) set" where
@@ -149,20 +181,476 @@ definition sems ::
  * might be easier than dealing with the details of
  * using automation to construct proofs out of the locale instances.
  *)
+(* YOU ARE HERE
+ * i think the problem is with the skip case of calc. we would need to know that it isn't that case
+ * that still doesn't answer why mem would be greater though...? *)
+(*
 lemma calc_dom_mem :
   "dominant2 calc_lift calc_trans mem_lift mem_trans { x . case x of (Sc _) \<Rightarrow> True | _ \<Rightarrow> False}"
 proof(rule dominant2.intro)
-  fix a1 a2 b x
-
+  fix a1 a2 x
+  fix b :: "(_, (_ :: {Okay, Mergeableb, Bogus})) state"
+  term "b"
+  term "LUpd mem_lift"
   assume X: "x \<in> {x. case x of Calc_Mem_Imp.syn.Sc x \<Rightarrow> True
                 | _ \<Rightarrow> False}"
+  assume B_ok : "b \<in> ok_S"
   then show
     "LUpd mem_lift (Calc_Mem_Imp.mem_trans x) a2 b <[
-       LUpd calc_lift (Calc_Mem_Imp.calc_trans x) a1 b"
+       LUpd calc_lift (Calc_Mem_Imp.calc_trans x) a1 b" using X
   unfolding calc_lift_def calc_schemi_def calc_schemo_def
             mem_lift_def mem_lift1_def no_control_lifting_def schem_lift_defs
   apply(auto simp add: schem_lift_defs lifter_instances
+  prod_ok_S prio_ok_S option_ok_S triv_ok_S
+prod_pleq leq_refl
  split: prod.splits md_prio.splits syn.splits option.splits)
+*)
+
+lemma calc_dom_mem :
+  "(with_baseline calc_sem_l) \<downharpoonleft> {with_baseline mem_sem_l, with_baseline calc_sem_l} { x . case x of (Sc _) \<Rightarrow> True | _ \<Rightarrow> False}"
+proof
+  fix b :: "(_, (_ :: {Bogus, Mergeableb})) state"
+  fix x
+  assume Xin : "x \<in> {x. case x of Sc x \<Rightarrow> True
+                   | _ \<Rightarrow> False} "
+  assume Bin : "b \<in> ok_S"
+  show "
+           is_sup
+            ((\<lambda>g. g x b) `
+             {with_baseline mem_sem_l,
+              with_baseline calc_sem_l})
+            (with_baseline calc_sem_l x b)"
+  proof(simp; rule is_sup_pair)
+    show "with_baseline mem_sem_l x b <[
+    with_baseline calc_sem_l x b"
+      using Xin Bin
+  unfolding calc_lift_def calc_schemi_def calc_schemo_def
+            mem_lift_def mem_lift1_def no_control_lifting_def schem_lift_defs with_baseline_def
+mem_sem_l_def calc_sem_l_def baseline_l_def baseline_f_def
+       apply(auto split: prod.splits md_prio.splits option.splits syn.splits md_triv.splits)
+    by(auto simp add: schem_lift_defs lifter_instances
+    prod_ok_S prio_ok_S option_ok_S triv_ok_S
+  prio_pleq triv_pleq
+  prod_pleq leq_refl lift_map_s_def option_pleq
+  prod_bsup prio_bsup option_bsup triv_bsup schem_lift_defs
+split: option.splits md_triv.splits prod.splits)
+qed
+qed
+
+lemma calc_dom_cond :
+  "(with_baseline calc_sem_l) \<downharpoonleft> {with_baseline cond_sem_l, with_baseline calc_sem_l} { x . case x of (Sc _) \<Rightarrow> True | _ \<Rightarrow> False}"
+proof
+  fix b :: "(_, (_ :: {Bogus, Mergeableb})) state"
+  fix x
+  assume Xin : "x \<in> {x. case x of Sc x \<Rightarrow> True
+                   | _ \<Rightarrow> False} "
+  assume Bin : "b \<in> ok_S"
+  show "is_sup
+            ((\<lambda>g. g x b) `
+             {with_baseline cond_sem_l,
+              with_baseline calc_sem_l})
+            (with_baseline calc_sem_l x b)"
+  proof(simp; rule is_sup_pair)
+    show "with_baseline cond_sem_l x b <[
+    with_baseline calc_sem_l x b"
+      using Xin Bin
+  unfolding calc_lift_def calc_schemi_def calc_schemo_def
+            mem_lift_def mem_lift1_def no_control_lifting_def schem_lift_defs with_baseline_def
+mem_sem_l_def calc_sem_l_def cond_sem_l_def baseline_l_def baseline_f_def cond_lift_def cond_sem_def
+       apply(auto split: prod.splits md_prio.splits option.splits syn.splits md_triv.splits)
+  by(auto simp add: schem_lift_defs lifter_instances
+    prod_ok_S prio_ok_S option_ok_S triv_ok_S
+  prio_pleq triv_pleq
+  prod_pleq leq_refl lift_map_s_def option_pleq
+  prod_bsup prio_bsup option_bsup triv_bsup schem_lift_defs
+split: option.splits md_triv.splits prod.splits)
+qed
+qed
+
+
+lemma calc_dom_imp :
+  "(with_baseline calc_sem_l) \<downharpoonleft> {with_baseline imp_sem_l, with_baseline calc_sem_l} { x . case x of (Sc _) \<Rightarrow> True | _ \<Rightarrow> False}"
+proof
+  fix b :: "(_, (_ :: {Bogus, Mergeableb, Okay, Pordc_all})) state"
+  fix x
+  assume Xin : "x \<in> {x. case x of Sc x \<Rightarrow> True
+                   | _ \<Rightarrow> False} "
+  assume Bin : "b \<in> ok_S"
+  show "is_sup
+            ((\<lambda>g. g x b) `
+             {with_baseline imp_sem_l,
+              with_baseline calc_sem_l})
+            (with_baseline calc_sem_l x b)"
+  proof(simp; rule is_sup_pair)
+    show "with_baseline imp_sem_l x b <[
+    with_baseline calc_sem_l x b"
+      using Xin Bin
+  unfolding calc_lift_def calc_schemi_def calc_schemo_def
+            mem_lift_def mem_lift1_def no_control_lifting_def schem_lift_defs with_baseline_def
+mem_sem_l_def calc_sem_l_def cond_sem_l_def baseline_l_def baseline_f_def cond_lift_def cond_sem_def
+imp_sem_l_def imp_sem_l_gen_def lift_map_s_def imp_ctl_sem_def get_cond_def imp_sem_lifting_gen_def
+       apply(auto split: prod.splits md_prio.splits option.splits syn.splits md_triv.splits list.splits)
+  by(auto simp add: schem_lift_defs lifter_instances
+    prod_ok_S prio_ok_S option_ok_S triv_ok_S
+  prio_pleq triv_pleq
+  prod_pleq leq_refl lift_map_s_def option_pleq
+  prod_bsup prio_bsup option_bsup triv_bsup schem_lift_defs imp_prio_def
+split: option.splits md_triv.splits prod.splits list.splits 
+)
+
+qed
+qed
+(*
+lemma calc_dom_seq :
+  "(with_baseline calc_sem_l) \<downharpoonleft> {with_baseline seq_sem_l, with_baseline calc_sem_l} { x . case x of (Sc _) \<Rightarrow> True | _ \<Rightarrow> False}"
+proof
+  fix b :: "(_, (_ :: {Bogus, Mergeableb, Okay})) state"
+  fix x
+  assume Xin : "x \<in> {x. case x of Sc x \<Rightarrow> True
+                   | _ \<Rightarrow> False} "
+  assume Bin : "b \<in> ok_S"
+  show "is_sup
+            ((\<lambda>g. g x b) `
+             {with_baseline seq_sem_l,
+              with_baseline calc_sem_l})
+            (with_baseline calc_sem_l x b)"
+  proof(simp; rule is_sup_pair)
+    show "with_baseline seq_sem_l x b <[
+    with_baseline calc_sem_l x b"
+      using Xin Bin
+  unfolding calc_lift_def calc_schemi_def calc_schemo_def
+            mem_lift_def mem_lift1_def no_control_lifting_def schem_lift_defs with_baseline_def
+mem_sem_l_def calc_sem_l_def cond_sem_l_def baseline_l_def baseline_f_def cond_lift_def cond_sem_def
+imp_sem_l_def imp_sem_l_gen_def lift_map_s_def imp_ctl_sem_def get_cond_def imp_sem_lifting_gen_def
+seq_sem_l_def seq_sem_l_gen_def seq_sem_lifting_gen_def
+       apply(auto split: prod.splits md_prio.splits option.splits syn.splits md_triv.splits list.splits)
+  apply(auto simp add: schem_lift_defs lifter_instances
+    prod_ok_S prio_ok_S option_ok_S triv_ok_S
+  prio_pleq triv_pleq
+  prod_pleq leq_refl lift_map_s_def option_pleq
+  prod_bsup prio_bsup option_bsup triv_bsup schem_lift_defs imp_prio_def
+split: option.splits md_triv.splits prod.splits list.splits 
+)
+*)
+
+lemma mem_dom_calc :
+  "(with_baseline mem_sem_l) \<downharpoonleft> {with_baseline calc_sem_l, with_baseline mem_sem_l} { x . case x of (Sm _) \<Rightarrow> True | _ \<Rightarrow> False}"
+proof
+  fix b :: "(_, (_ :: {Bogus, Mergeableb, Okay})) state"
+  fix x
+  assume Xin : "x \<in> {x. case x of Sm x \<Rightarrow> True
+                   | _ \<Rightarrow> False} "
+  assume Bin : "b \<in> ok_S"
+  show "is_sup
+            ((\<lambda>g. g x b) `
+             {with_baseline calc_sem_l,
+              with_baseline mem_sem_l})
+            (with_baseline mem_sem_l x b)"
+  proof(simp; rule is_sup_pair)
+    show "with_baseline calc_sem_l x b <[
+    with_baseline mem_sem_l x b"
+      using Xin Bin
+  unfolding calc_lift_def calc_schemi_def calc_schemo_def
+            mem_lift_def mem_lift1_def no_control_lifting_def schem_lift_defs with_baseline_def
+mem_sem_l_def calc_sem_l_def cond_sem_l_def baseline_l_def baseline_f_def cond_lift_def cond_sem_def
+imp_sem_l_def imp_sem_l_gen_def lift_map_s_def imp_ctl_sem_def get_cond_def imp_sem_lifting_gen_def
+seq_sem_l_def seq_sem_l_gen_def seq_sem_lifting_gen_def
+       apply(auto split: prod.splits md_prio.splits option.splits syn.splits md_triv.splits list.splits)
+  apply(auto simp add: schem_lift_defs lifter_instances
+    prod_ok_S prio_ok_S option_ok_S triv_ok_S
+  prio_pleq triv_pleq
+  prod_pleq leq_refl lift_map_s_def option_pleq
+  prod_bsup prio_bsup option_bsup triv_bsup schem_lift_defs imp_prio_def
+split: option.splits md_triv.splits prod.splits list.splits )
+  done
+qed
+qed
+
+lemma mem_dom_cond :
+  "(with_baseline mem_sem_l) \<downharpoonleft> {with_baseline cond_sem_l, with_baseline mem_sem_l} { x . case x of (Sm _) \<Rightarrow> True | _ \<Rightarrow> False}"
+proof
+  fix b :: "(_, (_ :: {Bogus, Mergeableb, Okay})) state"
+  fix x
+  assume Xin : "x \<in> {x. case x of Sm x \<Rightarrow> True
+                   | _ \<Rightarrow> False} "
+  assume Bin : "b \<in> ok_S"
+  show "is_sup
+            ((\<lambda>g. g x b) `
+             {with_baseline cond_sem_l,
+              with_baseline mem_sem_l})
+            (with_baseline mem_sem_l x b)"
+  proof(simp; rule is_sup_pair)
+    show "with_baseline cond_sem_l x b <[
+    with_baseline mem_sem_l x b"
+      using Xin Bin
+  unfolding calc_lift_def calc_schemi_def calc_schemo_def
+            mem_lift_def mem_lift1_def no_control_lifting_def schem_lift_defs with_baseline_def
+mem_sem_l_def calc_sem_l_def cond_sem_l_def baseline_l_def baseline_f_def cond_lift_def cond_sem_def
+imp_sem_l_def imp_sem_l_gen_def lift_map_s_def imp_ctl_sem_def get_cond_def imp_sem_lifting_gen_def
+seq_sem_l_def seq_sem_l_gen_def seq_sem_lifting_gen_def
+       apply(auto split: prod.splits md_prio.splits option.splits syn.splits md_triv.splits list.splits)
+  apply(auto simp add: schem_lift_defs lifter_instances
+    prod_ok_S prio_ok_S option_ok_S triv_ok_S
+  prio_pleq triv_pleq
+  prod_pleq leq_refl lift_map_s_def option_pleq
+  prod_bsup prio_bsup option_bsup triv_bsup schem_lift_defs imp_prio_def
+split: option.splits md_triv.splits prod.splits list.splits )
+  done
+qed
+qed
+
+lemma mem_dom_imp :
+  "(with_baseline mem_sem_l) \<downharpoonleft> {with_baseline imp_sem_l, with_baseline mem_sem_l} { x . case x of (Sm _) \<Rightarrow> True | _ \<Rightarrow> False}"
+proof
+  fix b :: "(_, (_ :: {Bogus, Mergeableb, Okay, Pordc_all})) state"
+  fix x
+  assume Xin : "x \<in> {x. case x of Sm x \<Rightarrow> True
+                   | _ \<Rightarrow> False} "
+  assume Bin : "b \<in> ok_S"
+  show "is_sup
+            ((\<lambda>g. g x b) `
+             {with_baseline imp_sem_l,
+              with_baseline mem_sem_l})
+            (with_baseline mem_sem_l x b)"
+  proof(simp; rule is_sup_pair)
+    show "with_baseline imp_sem_l x b <[
+    with_baseline mem_sem_l x b"
+      using Xin Bin
+  unfolding calc_lift_def calc_schemi_def calc_schemo_def
+            mem_lift_def mem_lift1_def no_control_lifting_def schem_lift_defs with_baseline_def
+mem_sem_l_def calc_sem_l_def cond_sem_l_def baseline_l_def baseline_f_def cond_lift_def cond_sem_def
+imp_sem_l_def imp_sem_l_gen_def lift_map_s_def imp_ctl_sem_def get_cond_def imp_sem_lifting_gen_def
+seq_sem_l_def seq_sem_l_gen_def seq_sem_lifting_gen_def
+       apply(auto split: prod.splits md_prio.splits option.splits syn.splits md_triv.splits list.splits)
+  apply(auto simp add: schem_lift_defs lifter_instances
+    prod_ok_S prio_ok_S option_ok_S triv_ok_S
+  prio_pleq triv_pleq
+  prod_pleq leq_refl lift_map_s_def option_pleq
+  prod_bsup prio_bsup option_bsup triv_bsup schem_lift_defs imp_prio_def
+split: option.splits md_triv.splits prod.splits list.splits )
+  done
+qed
+qed
+
+lemma cond_dom_calc :
+  "(with_baseline cond_sem_l) \<downharpoonleft> {with_baseline calc_sem_l, with_baseline cond_sem_l} { x . case x of (Sb _) \<Rightarrow> True | _ \<Rightarrow> False}"
+proof
+  fix b :: "(_, (_ :: {Bogus, Mergeableb, Okay})) state"
+  fix x
+  assume Xin : "x \<in> {x. case x of Sb x \<Rightarrow> True
+                   | _ \<Rightarrow> False} "
+  assume Bin : "b \<in> ok_S"
+  show "is_sup
+            ((\<lambda>g. g x b) `
+             {with_baseline calc_sem_l,
+              with_baseline cond_sem_l})
+            (with_baseline cond_sem_l x b)"
+  proof(simp; rule is_sup_pair)
+    show "with_baseline calc_sem_l x b <[
+    with_baseline cond_sem_l x b"
+      using Xin Bin
+  unfolding calc_lift_def calc_schemi_def calc_schemo_def
+            mem_lift_def mem_lift1_def no_control_lifting_def schem_lift_defs with_baseline_def
+mem_sem_l_def calc_sem_l_def cond_sem_l_def baseline_l_def baseline_f_def cond_lift_def cond_sem_def
+imp_sem_l_def imp_sem_l_gen_def lift_map_s_def imp_ctl_sem_def get_cond_def imp_sem_lifting_gen_def
+seq_sem_l_def seq_sem_l_gen_def seq_sem_lifting_gen_def
+       apply(auto split: prod.splits md_prio.splits option.splits syn.splits md_triv.splits list.splits)
+  apply(auto simp add: schem_lift_defs lifter_instances
+    prod_ok_S prio_ok_S option_ok_S triv_ok_S
+  prio_pleq triv_pleq
+  prod_pleq leq_refl lift_map_s_def option_pleq
+  prod_bsup prio_bsup option_bsup triv_bsup schem_lift_defs imp_prio_def
+split: option.splits md_triv.splits prod.splits list.splits )
+  done
+qed
+qed
+
+lemma cond_dom_mem :
+  "(with_baseline cond_sem_l) \<downharpoonleft> {with_baseline mem_sem_l, with_baseline cond_sem_l} { x . case x of (Sb _) \<Rightarrow> True | _ \<Rightarrow> False}"
+proof
+  fix b :: "(_, (_ :: {Bogus, Mergeableb, Okay})) state"
+  fix x
+  assume Xin : "x \<in> {x. case x of Sb x \<Rightarrow> True
+                   | _ \<Rightarrow> False} "
+  assume Bin : "b \<in> ok_S"
+  show "is_sup
+            ((\<lambda>g. g x b) `
+             {with_baseline mem_sem_l,
+              with_baseline cond_sem_l})
+            (with_baseline cond_sem_l x b)"
+  proof(simp; rule is_sup_pair)
+    show "with_baseline mem_sem_l x b <[
+    with_baseline cond_sem_l x b"
+      using Xin Bin
+  unfolding calc_lift_def calc_schemi_def calc_schemo_def
+            mem_lift_def mem_lift1_def no_control_lifting_def schem_lift_defs with_baseline_def
+mem_sem_l_def calc_sem_l_def cond_sem_l_def baseline_l_def baseline_f_def cond_lift_def cond_sem_def
+imp_sem_l_def imp_sem_l_gen_def lift_map_s_def imp_ctl_sem_def get_cond_def imp_sem_lifting_gen_def
+seq_sem_l_def seq_sem_l_gen_def seq_sem_lifting_gen_def
+       apply(auto split: prod.splits md_prio.splits option.splits syn.splits md_triv.splits list.splits)
+  apply(auto simp add: schem_lift_defs lifter_instances
+    prod_ok_S prio_ok_S option_ok_S triv_ok_S
+  prio_pleq triv_pleq
+  prod_pleq leq_refl lift_map_s_def option_pleq
+  prod_bsup prio_bsup option_bsup triv_bsup schem_lift_defs imp_prio_def
+split: option.splits md_triv.splits prod.splits list.splits )
+  done
+qed
+qed
+
+lemma cond_dom_imp :
+  "(with_baseline cond_sem_l) \<downharpoonleft> {with_baseline imp_sem_l, with_baseline cond_sem_l} { x . case x of (Sb _) \<Rightarrow> True | _ \<Rightarrow> False}"
+proof
+  fix b :: "(_, (_ :: {Bogus, Mergeableb, Okay, Pordc_all})) state"
+  fix x
+  assume Xin : "x \<in> {x. case x of Sb x \<Rightarrow> True
+                   | _ \<Rightarrow> False} "
+  assume Bin : "b \<in> ok_S"
+  show "is_sup
+            ((\<lambda>g. g x b) `
+             {with_baseline imp_sem_l,
+              with_baseline cond_sem_l})
+            (with_baseline cond_sem_l x b)"
+  proof(simp; rule is_sup_pair)
+    show "with_baseline imp_sem_l x b <[
+    with_baseline cond_sem_l x b"
+      using Xin Bin
+  unfolding calc_lift_def calc_schemi_def calc_schemo_def
+            mem_lift_def mem_lift1_def no_control_lifting_def schem_lift_defs with_baseline_def
+mem_sem_l_def calc_sem_l_def cond_sem_l_def baseline_l_def baseline_f_def cond_lift_def cond_sem_def
+imp_sem_l_def imp_sem_l_gen_def lift_map_s_def imp_ctl_sem_def get_cond_def imp_sem_lifting_gen_def
+seq_sem_l_def seq_sem_l_gen_def seq_sem_lifting_gen_def
+       apply(auto split: prod.splits md_prio.splits option.splits syn.splits md_triv.splits list.splits)
+  apply(auto simp add: schem_lift_defs lifter_instances
+    prod_ok_S prio_ok_S option_ok_S triv_ok_S
+  prio_pleq triv_pleq
+  prod_pleq leq_refl lift_map_s_def option_pleq
+  prod_bsup prio_bsup option_bsup triv_bsup schem_lift_defs imp_prio_def
+split: option.splits md_triv.splits prod.splits list.splits )
+  done
+qed
+qed
+
+lemma imp_dom_calc :
+  "(with_baseline imp_sem_l) \<downharpoonleft> {with_baseline calc_sem_l, with_baseline imp_sem_l} { x . case x of (Si _) \<Rightarrow> True | _ \<Rightarrow> False}"
+proof
+  fix b :: "(_, (_ :: {Bogus, Mergeableb, Okay, Pordc_all})) state"
+  fix x
+  assume Xin : "x \<in> {x. case x of Si x \<Rightarrow> True
+                   | _ \<Rightarrow> False} "
+  assume Bin : "b \<in> ok_S"
+  show "is_sup
+            ((\<lambda>g. g x b) `
+             {with_baseline calc_sem_l,
+              with_baseline imp_sem_l})
+            (with_baseline imp_sem_l x b)"
+  proof(simp; rule is_sup_pair)
+    show "with_baseline calc_sem_l x b <[
+    with_baseline imp_sem_l x b"
+      using Xin Bin
+  unfolding calc_lift_def calc_schemi_def calc_schemo_def
+            mem_lift_def mem_lift1_def no_control_lifting_def schem_lift_defs with_baseline_def
+mem_sem_l_def calc_sem_l_def cond_sem_l_def baseline_l_def baseline_f_def cond_lift_def cond_sem_def
+imp_sem_l_def imp_sem_l_gen_def lift_map_s_def imp_ctl_sem_def get_cond_def imp_sem_lifting_gen_def
+seq_sem_l_def seq_sem_l_gen_def seq_sem_lifting_gen_def
+       apply(auto split: prod.splits md_prio.splits option.splits syn.splits md_triv.splits list.splits)
+  apply(auto simp add: schem_lift_defs lifter_instances
+    prod_ok_S prio_ok_S option_ok_S triv_ok_S
+  prio_pleq triv_pleq
+  prod_pleq leq_refl lift_map_s_def option_pleq
+  prod_bsup prio_bsup option_bsup triv_bsup schem_lift_defs imp_prio_def
+split: option.splits md_triv.splits prod.splits list.splits )
+  done
+qed
+qed
+
+lemma imp_dom_mem :
+  "(with_baseline imp_sem_l) \<downharpoonleft> {with_baseline mem_sem_l, with_baseline imp_sem_l} { x . case x of (Si _) \<Rightarrow> True | _ \<Rightarrow> False}"
+proof
+  fix b :: "(_, (_ :: {Bogus, Mergeableb, Okay, Pordc_all})) state"
+  fix x
+  assume Xin : "x \<in> {x. case x of Si x \<Rightarrow> True
+                   | _ \<Rightarrow> False} "
+  assume Bin : "b \<in> ok_S"
+  show "is_sup
+            ((\<lambda>g. g x b) `
+             {with_baseline mem_sem_l,
+              with_baseline imp_sem_l})
+            (with_baseline imp_sem_l x b)"
+  proof(simp; rule is_sup_pair)
+    show "with_baseline mem_sem_l x b <[
+    with_baseline imp_sem_l x b"
+      using Xin Bin
+  unfolding calc_lift_def calc_schemi_def calc_schemo_def
+            mem_lift_def mem_lift1_def no_control_lifting_def schem_lift_defs with_baseline_def
+mem_sem_l_def calc_sem_l_def cond_sem_l_def baseline_l_def baseline_f_def cond_lift_def cond_sem_def
+imp_sem_l_def imp_sem_l_gen_def lift_map_s_def imp_ctl_sem_def get_cond_def imp_sem_lifting_gen_def
+seq_sem_l_def seq_sem_l_gen_def seq_sem_lifting_gen_def
+       apply(auto split: prod.splits md_prio.splits option.splits syn.splits md_triv.splits list.splits)
+  apply(auto simp add: schem_lift_defs lifter_instances
+    prod_ok_S prio_ok_S option_ok_S triv_ok_S
+  prio_pleq triv_pleq
+  prod_pleq leq_refl lift_map_s_def option_pleq
+  prod_bsup prio_bsup option_bsup triv_bsup schem_lift_defs imp_prio_def
+split: option.splits md_triv.splits prod.splits list.splits )
+  done
+qed
+qed
+
+
+lemma imp_dom_cond :
+  "(with_baseline imp_sem_l) \<downharpoonleft> {with_baseline cond_sem_l, with_baseline imp_sem_l} { x . case x of (Si _) \<Rightarrow> True | _ \<Rightarrow> False}"
+proof
+  fix b :: "(_, (_ :: {Bogus, Mergeableb, Okay, Pordc_all})) state"
+  fix x
+  assume Xin : "x \<in> {x. case x of Si x \<Rightarrow> True
+                   | _ \<Rightarrow> False} "
+  assume Bin : "b \<in> ok_S"
+  show "is_sup
+            ((\<lambda>g. g x b) `
+             {with_baseline cond_sem_l,
+              with_baseline imp_sem_l})
+            (with_baseline imp_sem_l x b)"
+  proof(simp; rule is_sup_pair)
+    show "with_baseline cond_sem_l x b <[
+    with_baseline imp_sem_l x b"
+      using Xin Bin
+  unfolding calc_lift_def calc_schemi_def calc_schemo_def
+            mem_lift_def mem_lift1_def no_control_lifting_def schem_lift_defs with_baseline_def
+mem_sem_l_def calc_sem_l_def cond_sem_l_def baseline_l_def baseline_f_def cond_lift_def cond_sem_def
+imp_sem_l_def imp_sem_l_gen_def lift_map_s_def imp_ctl_sem_def get_cond_def imp_sem_lifting_gen_def
+seq_sem_l_def seq_sem_l_gen_def seq_sem_lifting_gen_def
+       apply(auto split: prod.splits md_prio.splits option.splits syn.splits md_triv.splits list.splits)
+  apply(auto simp add: schem_lift_defs lifter_instances
+    prod_ok_S prio_ok_S option_ok_S triv_ok_S
+  prio_pleq triv_pleq
+  prod_pleq leq_refl lift_map_s_def option_pleq
+  prod_bsup prio_bsup option_bsup triv_bsup schem_lift_defs imp_prio_def
+split: option.splits md_triv.splits prod.splits list.splits )
+  done
+qed
+qed
+
+
+(*
+proof(rule dominant2.intro)
+  fix a1 a2 x
+  fix b :: "(_, (_ :: {Okay, Mergeableb, Bogus})) state"
+  term "b"
+  term "LUpd mem_lift"
+  assume X: "x \<in> {x. case x of Calc_Mem_Imp.syn.Sc x \<Rightarrow> True
+                | _ \<Rightarrow> False}"
+  assume B_ok : "b \<in> ok_S"
+  then show
+    "LUpd mem_lift (Calc_Mem_Imp.mem_trans x) a2 b <[
+       LUpd calc_lift (Calc_Mem_Imp.calc_trans x) a1 b" using X
+  unfolding calc_lift_def calc_schemi_def calc_schemo_def
+            mem_lift_def mem_lift1_def no_control_lifting_def schem_lift_defs
+  apply(auto simp add: schem_lift_defs lifter_instances
+  prod_ok_S prio_ok_S option_ok_S triv_ok_S
+prod_pleq leq_refl
+*)
+
 (*
   apply(simp)
   apply(rule dominant2_snd.ax)
